src/rocq/Semantics/InfiniteToFinite/R2Injective.v
@@ -1,3 +1,4 @@
+Unset Universe Checking.
 From Vellvm Require Import
   Semantics.TopLevel
   Utils.Tactics
