src/rocq/Theory/DenotationTheory.v
@@ -8,7 +8,7 @@ From ITree Require Import
      ITree
      ITreeFacts
      Basics.HeterogeneousRelations.
-
+Unset Universe Checking.
 From Vellvm Require Import
      Utilities
      Syntax
