src/rocq/Theory/ExpLemmas.v
@@ -17,7 +17,7 @@ From ITree Require Import
      Interp.InterpFacts
      Events.State
      Events.StateFacts.
-
+Unset Universe Checking.
 From Vellvm Require Import
      Utilities
      Syntax
