src/rocq/Theory/InstrLemmas.v
@@ -10,13 +10,14 @@ From ITree Require Import
      Basics.Monad
      Eq.Eqit
      TranslateFacts.
-
+Unset Universe Checking.
 From Vellvm Require Import
      Utilities
      Utils.MapMonadExtra
      Semantics
-     Theory.InterpreterCFG.
-
+     Theory.InterpreterCFG
+     LLVMAst.
+From ExtLib Require Import Structures.Functor.
 Open Scope list_scope.
 Open Scope itree_scope.
 
@@ -121,28 +122,610 @@ Module InstrLemmas (IS : InterpreterStack) (TOP : LLVMTopLevel IS).
   End InstrTactics.
 
   Import InstrTactics.
+    (* RJS 10 Mar:
+      1. Let's do symbolic stepping over the following instructions:
+        Op
+        Load
+        Store
+        Alloca
+      
+      2. Multi-instruction steps, i.e. if we have store-load,
+       and the loaded pointer is no longer live, can we turn that into just the register value?
+
+      3. A 'swap instruction' lemma along the lines of swapping two loads or a load and a store
+       if they are of different memory locations and to different registers.
+      
+      4. denote_function: How do I say that two functions are equivalent for any input
+        that is, they have the same set of external effects and the same return value,
+        at the denote function level.
+      
+      5. cfg-mcfg link: To show that two functions are equivalent,
+       should we be using interp_cfgn_exec, interp_cfgn, interp_mcfgn_exec, or interp_mcfgn?
+
+      6. What would an alternate 'error-absorbing' interp for levels 4-6 look like that would allow us to always have a Ret,
+        allowing Program Definition based approach to defining instruction rewriting lemmas. 
+      
+      *)
+      (* Lemma eval_int_op_err_ub_oom_to_itree :
+      forall {E} `{OOME -< E} `{FailureE -< E} `{UBE -< E} {I} `{VMI : VellvmIntegers.VMemInt I} `{DVI : ToDvalue I}
+        x y iop,
+        (@eval_int_op (itree E) I _ _ _ _ _ _ iop x y) ≈
+          match eval_int_op iop x y with
+          | ERR_UB_OOM (mkEitherT (mkEitherT (mkEitherT (mkIdent m)))) =>
+              match m with
+              | inl (OOM_message x) => raiseOOM x
+              | inr (inl (UB_message x)) => raiseUB x
+              | inr (inr (inl (ERR_message x))) => raise x
+              | inr (inr (inr x)) => ret x
+              end
+          end.
+    Proof.
+      intros E H H0 H1 I VMI DVI x y iop.
+      unfold eval_int_op.
+      destruct iop; cbn; try reflexivity;
+        try solve
+          [ break_match; reflexivity
+          | break_match; cbn; try reflexivity;
+            unfold lift_OOM;
+            break_inner_match; cbn;
+            process;
+            try reflexivity
+          | break_match; cbn; try reflexivity;
+            unfold lift_OOM;
+            break_inner_match; cbn;
+            process;
+            try reflexivity;
+            setoid_rewrite IP.VMemInt_intptr_dtyp;
+            setoid_rewrite dtyp_eqb_refl;
+            break_match; cbn; reflexivity
+          ].
+      - break_match; cbn; try reflexivity;
+          unfold lift_OOM;
+          break_inner_match; cbn;
+          process; try reflexivity.
+        repeat (break_match; cbn; try reflexivity);
+          process; try reflexivity.
+      - break_match; cbn; try reflexivity;
+          unfold lift_OOM;
+          break_inner_match; cbn;
+          process; try reflexivity.
+        repeat (break_match; cbn; try reflexivity);
+          process; try reflexivity.
+        repeat (break_match; cbn; try reflexivity);
+          repeat rewrite bind_ret_l; try reflexivity;
+          try discriminate.
+        all: try (subst; cbn in *;
+                  rewrite Heqb3;
+                  inv Heqi1;
+                  reflexivity).
+        all: (repeat (break_match; cbn; try reflexivity);
+              repeat setoid_rewrite Raise.raiseOOM_bind_itree; reflexivity).
+      - break_match; cbn; try reflexivity;
+          unfold lift_OOM;
+          break_inner_match; cbn;
+          process; try reflexivity.
+        repeat (break_match; cbn; try reflexivity);
+          process; try reflexivity.
+      - break_match; cbn; try reflexivity;
+          unfold lift_OOM;
+          break_inner_match; cbn;
+          process; try reflexivity.
+        repeat (break_match; cbn; try reflexivity);
+          process; try reflexivity.
+      - break_match; cbn; try reflexivity;
+          unfold lift_OOM;
+          break_inner_match; cbn;
+          process; try reflexivity.
+        repeat (break_match; cbn; try reflexivity);
+          process; try reflexivity.
+    Qed. *)
 
   (* Note: we know that we can prove that [l = l'] is always true.
    However there is no reason to put this burden on the hypothesis, it is easier to use this way.
    Arguably we could do the same for [g] and [m] but haven't felt the need for it so far.
    *)
-  (* Lemma denote_instr_load : *)
-  (*   forall (i : raw_id) volatile τ τp ptr align g l l' m a uv, *)
-  (*     ⟦ ptr at τp ⟧e3 g l m ≈ Ret3 g l' m (UVALUE_Addr a) -> *)
-  (*     read m a τ = inr uv -> *)
-  (*     ⟦ (IId i, INSTR_Load volatile τ (τp, ptr) align) ⟧i3 g l m ≈ Ret3 g (Maps.add i uv l') m tt. *)
-  (* Proof. *)
-  (*   intros * EXP READ. *)
-  (*   cbn. *)
-  (*   go. *)
-  (*   rewrite EXP. *)
-  (*   go. *)
-  (*   cbn. *)
-  (*   go. *)
-  (*   step. *)
-  (*   step. *)
-  (*   reflexivity. *)
-  (* Qed. *)
+   (* Need to put the result of eval_int_op into the environment. *)
+   (* Check interp_cfg2.
+   Section dostuff.
+    Variable u: @Integers.bit_int 64.
+    Variable _id: raw_id.
+    Variable les: local_env.
+    Variable g: global_env.
+    Check (Integers.repr 5).
+      Check ((@eval_int_op _ _ _ _ _ _ _ _ (Add false true) u (Integers.repr 5%Z))).
+      Check @eval_int_op.
+      Locate eval_int_op.
+      Check @eval_int_op.
+
+
+
+Lemma interp3e_instr_op g les reg u  _id:
+    (FMapAList.alist_find (Anon reg%Z) les) = Some (@UVALUE_I 64 u) ->
+    (* contains_undef_or_poison u = false ->  *)
+    eutt eq (interp_cfg2 (⟦ (IId _id,
+                              INSTR_Op (OP_IBinop (LLVMAst.Add false true)
+                                          (DynamicTypes.DTYPE_I 64) (EXP_Ident (ID_Local (Anon (reg)%Z))) (EXP_Integer (5)%Z))) ⟧i None) g les)
+      (fmap (fun res => (FMapAList.alist_add _id (dvalue_to_uvalue res) les, (g, tt))) (@eval_int_op _ _ _ _ _ _ ((@VellvmIntegers.VIntVMemInt (@Integers.bit_int 64) (VellvmIntegers.VInt_Bounded 64))) _ (Add false true) u (Integers.repr 5%Z))).
+   Proof.
+
+  Check (fmap (fun res => (FMapAList.alist_add _id (dvalue_to_uvalue res) les, (g, tt))) (@eval_int_op (itree L2) _ _ _ _ _ _ _ (Add false true) u (Integers.repr 5%Z))). *)
+  (* Import LLVMParamsBigIntptr.Events.DV. *)
+Require Import ZArith.
+Print local_env.
+Lemma interp2_instr_op g les u _id x:
+    (FMapAList.alist_find x les) = Some (@UVALUE_I 64 u) ->
+    (* contains_undef_or_poison u = false ->  *)
+    eutt eq (interp_cfg2 (⟦ (IId _id,
+                              INSTR_Op (OP_IBinop (LLVMAst.Add false true)
+                                          (DynamicTypes.DTYPE_I 64) (EXP_Ident (ID_Local x)) (EXP_Integer (5)%Z))) ⟧i None) g les)
+      (fmap (fun res => (FMapAList.alist_add _id (dvalue_to_uvalue res) les, (g, tt))) (@eval_int_op _ _ _ _ _ _ ((@VellvmIntegers.VIntVMemInt (@Integers.bit_int 64) (VellvmIntegers.VInt_Bounded 64))) _ (Add false true) u (Integers.repr 5%Z))).
+Proof.
+  Local Opaque eval_int_op.
+  intros Hfind .
+  cbn.
+  Ltac step :=  lazymatch goal with 
+  | |- _ (interp_cfg2 (_ <- _ ;; _ ) _ _) _ => rewrite interp_cfg2_bind
+  | |- _ (interp_cfg2 (translate _ (_ <- _ ;; _ )) _ _) _ => rewrite translate_bind
+  | |- _ (_ <- (interp_cfg2 (_ <- _ ;; _ ) _ _);; _) _ => rewrite interp_cfg2_bind
+  | |- _ (_ <- (interp_cfg2 (translate _ (_ <- _ ;; _ )) _ _);; _) _ => rewrite translate_bind
+  | |- _ (_ <- (interp_cfg2 (translate _ (ITree.map _ _)) _ _);; _) _ => unfold ITree.map
+  | |- _ (_ <- (interp_cfg2 (translate _ (Ret _)) _ _);; _) _ => rewrite translate_ret
+  | |- _ (_ <- (interp_cfg2 (translate _ (raiseOOM _)) _ _);; _) _ => unfold raiseOOM; rewrite bind_trigger
+  | |- _ (_ <- (interp_cfg2 (translate _ (raiseUB _)) _ _);; _) _  => unfold raiseUB; rewrite bind_trigger
+  | |- _ (_ <- (interp_cfg2 (translate _ (raise _)) _ _);; _) _    => unfold raise; rewrite bind_trigger
+  | |- _ (_ <- (interp_cfg2 (translate _ (vis _ _)) _ _);; _) _    => rewrite translate_vis
+  | |- _ (_ <- (interp_cfg2 (vis _ _) _ _);; _) _    => rewrite interp_cfg2_vis
+  | |- _ (_ <- (interp_cfg2 (Vis _ _) _ _);; _) _    => rewrite interp_cfg2_vis
+  | |- _ (_ <- (interp_cfg2 (Ret _) _ _);; _) _ => rewrite interp_cfg2_ret
+  | |- _ (_ <- (interp_cfg2 (translate _ (translate _ _)) _ _);; _) _ => go; cbn
+  | |- _ (_ <- (interp_cfg2 (trigger (exp_to_instr _) ) _ _);; _) _ => unfold exp_to_instr; process
+  | |- _ (_ <- (interp_cfg2 (trigger (LocalRead _) ) _ _);; _) _ => rewrite interp_cfg2_LR
+  | |- _ (_ <- (_ <- _;; _) ;; _) _ => rewrite bind_bind
+  | |- _ (_ <- (trigger _) ;; _) _ => rewrite bind_trigger
+  | |- _ (_ <- (vis _ _) ;; _) _ => rewrite bind_vis
+  | |- _ (_ <- (Ret _);; _) _ => rewrite bind_ret_l
+  | |- _ => cbn
+  end.
+  repeat step.
+  2: apply Hfind.
+  cbn.
+  repeat step.
+  
+  
+  (* Local Opaque eval_iop. *)
+  repeat rewrite eval_int_op_err_ub_oom_to_itree.
+  remember (eval_int_op (Add false true) u (Integers.repr 5)) as x.
+  destruct_err_ub_oom x.
+  {
+    repeat step. 
+    process.
+    setoid_rewrite interp_cfg2_OOM.
+    repeat step.
+    rewrite bind_trigger.
+    rewrite bind_vis.
+    eapply eqit_Vis.
+    intros [].
+  }
+
+  { 
+    repeat step.
+    process.
+    setoid_rewrite interp_cfg2_UB.
+    repeat step.
+    rewrite bind_trigger.
+    rewrite bind_vis.
+    eapply eqit_Vis.
+    intros [].
+  }
+
+  { 
+    repeat step.
+    process.
+    setoid_rewrite interp_cfg2_Err.
+    repeat step.
+    rewrite bind_trigger.
+    rewrite bind_vis.
+    eapply eqit_Vis.
+    intros [].
+  }
+  repeat step.
+
+  rewrite interp_cfg2_LW.
+  cbn.
+  rewrite bind_ret_l.
+  reflexivity.
+Qed.
+Import VellvmRelations.
+From ITree Require Import RuttFacts.
+
+
+Definition instr_E_to_L0 {T : Type} : instr_E T -> itree L0 T :=
+fun (e : instr_E T) =>
+  match e with
+  | inl1 call =>
+      match call with
+      | Call dt fv args =>
+          raise "call"
+      end
+  | inr1 e0 =>
+      trigger e0
+  end.
+
+Definition interp_instr_E_to_L0 :=
+interp (@instr_E_to_L0).
+
+
+    (* forall t, 
+    (interp_cfg3 eq (⟦ (IId _id,
+                              INSTR_Op (OP_IBinop (LLVMAst.Add false true)
+                                          (DynamicTypes.DTYPE_I 64) (EXP_Ident (ID_Local (Anon (reg)%Z))) (EXP_Integer (5)%Z))) ⟧i None) g les sid mem
+      ) t 
+       <->
+    (MEM_SPEC_INTERP.interp_memory_spec eq 
+      (fmap (fun res => (FMapAList.alist_add _id (dvalue_to_uvalue res) les, (g, tt))) 
+        (@eval_int_op _ _ _ _ _ _ ((@VellvmIntegers.VIntVMemInt (@Integers.bit_int 64) (VellvmIntegers.VInt_Bounded 64))) _ (Add false true) u (Integers.repr 5%Z))) sid mem
+      ) t. *)
+Lemma interp3_instr_op reg u  _id g les sid mem:
+    (FMapAList.alist_find (Anon reg%Z) les) = Some (@UVALUE_I 64 u) ->
+    (* contains_undef_or_poison u = false ->  *)
+    refine_L3_cfg_eq (interp_cfg3 eq (⟦ (IId _id,
+                              INSTR_Op (OP_IBinop (LLVMAst.Add false true)
+                                          (DynamicTypes.DTYPE_I 64) (EXP_Ident (ID_Local (Anon (reg)%Z))) (EXP_Integer (5)%Z))) ⟧i None) g les sid mem
+      ) (MEM_SPEC_INTERP.interp_memory_spec eq 
+      (fmap (fun res => (FMapAList.alist_add _id (dvalue_to_uvalue res) les, (g, tt))) 
+        (@eval_int_op _ _ _ _ _ _ ((@VellvmIntegers.VIntVMemInt (@Integers.bit_int 64) (VellvmIntegers.VInt_Bounded 64))) _ (Add false true) u (Integers.repr 5%Z))) sid mem
+      ).
+Proof.
+  intros Hfind.
+  eapply refine_23_cfg_eq.
+  apply interp2_instr_op.
+  eauto.
+Qed.
+Import DynamicTypes.
+  Import IS.MEM.MEM_SPEC_INTERP.
+  (* #[global] Instance interp_cfg3_proper' {R}:
+      Proper (eutt eq ==> eq ==> eq ==> eq ==> eq ==> PropT.equiv_PropT) (@interp_cfg3 R eq).
+  Proof.
+    repeat red.
+    intros.
+    subst.
+  Admitted. *)
+
+  (* Polymorphic Instance Eq1_PropT {E} : Eq1 (PropT E) :=
+    fun a PA PA' =>
+      (forall x y, x ≈ y -> (PA x <-> PA' y)). *)
+
+
+    (* #[global] Instance interp_memory_spec_proper' {E R} {RR: R -> R -> Prop} :
+        Proper (eutt eq ==> eq ==> eq ==> eq ==> Basics.impl) (@interp_memory_spec E R R RR).
+    Proof.
+      Admitted. *)
+  Lemma interp_cfg3_LR' {RR} {EQR: Equivalence RR} : forall id g l sid mem v,
+      Maps.lookup id l = Some v ->
+      forall t1 t2,
+      eutt eq t1 t2 -> 
+      (* (interp_cfg3' RR (Ret v) g l sid mem) t -> *)
+      (interp_cfg3 RR (trigger (LocalRead id)) g l sid mem) t1
+      <->
+      (interp_cfg3 RR (Ret v) g l sid mem) t2.
+  Proof.
+    intros.
+    split.
+    unfold interp_cfg3.
+    intros.
+    rewrite interp_cfg2_LR in H1.
+    setoid_rewrite interp_cfg2_ret.
+    rewrite <- H0.
+    eauto.
+    eauto.
+    intros.
+    unfold interp_cfg3 in *.
+    rewrite interp_cfg2_LR.
+    setoid_rewrite interp_cfg2_ret in H1.
+    rewrite H0.
+    eauto.
+    eauto.
+  Qed.
+
+  (* #[global] Instance interp_cfg3_proper {R}:
+      Proper (eutt eq ==> iff ) (@interp_cfg3 R eq).
+  Proof.
+    admit.
+  Admitted. *)
+
+  (* #[global] Instance interp_cfg3_proper {R RR}:
+      Proper (eutt eq ==> eq ==> eq ==> eq ==> eq ==> eutt eq ==> iff ) (@interp_cfg3 R RR).
+  Proof.
+    admit.
+  Admitted. *)
+  Lemma interp_cfg3_LR {RR} {EQR: Equivalence RR} : forall id g l sid mem v,
+      Maps.lookup id l = Some v ->
+      (* (interp_cfg3' RR (Ret v) g l sid mem) t -> *)
+      Monad.eq1
+      (interp_cfg3 RR (trigger (LocalRead id)) g l sid mem)
+      (interp_cfg3 RR (Ret v) g l sid mem).
+  Proof.
+    intros.
+    repeat red.
+    split; intros; split; intros.
+    rewrite <- interp_cfg3_LR'; eauto.
+    rewrite interp_cfg3_LR'; eauto.
+
+    all: repeat red; intros; split; intros;
+      [try rewrite <- H0 | try rewrite H0]; eauto.
+  Qed.
+
+Notation PRet5 g l sid mem v:= (ret (mem, (sid, (l, (g, v))))).
+
+    (* Lemma interp_memory_spec_ret {R} {RR: R -> R -> Prop} sid ms r:
+      Monad.eq1
+      (interp_memory_spec RR (Ret r) sid ms)
+       (ret (ms, (sid, r))).
+    Proof using.
+    admit.
+    Admitted. *)
+  Lemma eq1_iff_propt {E R} (a b: PropT E R):
+    Monad.eq1 a b
+    ->
+    forall x,
+    a x <-> b x.
+  Proof.
+    intros.
+    destruct H.
+    apply H.
+    reflexivity.
+  Qed.
+
+Locate ret.
+   #[global] Instance ret_PropT_Proper {E R} :
+     Proper (eq ==> eutt eq ==> iff) (@ret (PropT E) _ R).
+   Proof using.
+   repeat red.
+   intros.
+   split;  cbn; intros; red; red; subst.
+   red in H1. red in H1.
+   rewrite <- H0. auto.
+   rewrite H0. auto.
+  Qed.
+
+  Lemma interp_cfg3_LR'' {RR} {EQR: Equivalence RR} : forall id g l sid mem v,
+      Maps.lookup id l = Some v ->
+      (* (interp_cfg3' RR (Ret v) g l sid mem) t -> *)
+      Monad.eq1
+      (interp_cfg3 RR (trigger (LocalRead id)) g l sid mem)
+       (* (eutt (eq × (eq × RR)) (ret (mem, (sid, (l, (g, v)))))). *)
+       (ret (mem, (sid, (l, (g, v))))).
+  Proof.
+    intros.
+    repeat red.
+    split;
+     intros; split; intros.
+    red in H1.
+
+    rewrite interp_cfg2_LR in H1; eauto.
+    epose proof interp_memory_spec_ret.
+    eapply eq1_iff_propt in H2.
+    apply H2.
+    rewrite <- H0.
+    eauto.
+
+    red.
+    rewrite interp_cfg2_LR; eauto.
+    rewrite H0.
+    epose proof interp_memory_spec_ret.
+    eapply eq1_iff_propt in H2.
+    apply H2.
+    eauto.
+
+    all: repeat red; intros; split; intros;
+      [try rewrite <- H0 | try rewrite H0]; eauto.
+  Qed.
+   #[global] Instance bind_PropT_Proper {E} {A B} :
+     Proper (eq1 ==> eq  ==> eq ==> iff) (@bind_PropT E A B).
+   Proof using.
+   Admitted.
+
+    (* Lemma interp_cfg3_ret'' {R} {RR} g les sid ms (r: R):
+      forall t,
+      (interp_cfg3 RR (Ret r) g les sid ms) t
+       <-> (eutt (eq × (eq × RR)) (ret (ms, (sid, (les, (g, r))))) t).
+    Proof using.
+    admit.
+    Admitted.
+    Lemma interp_cfg3_ret' {R} {RR} g les sid ms (r: R):
+      Monad.eq1
+      (interp_cfg3 RR (Ret r) g les sid ms) t
+       <-> (eutt (eq × (eq × RR)) (ret (ms, (sid, (les, (g, r))))) t).
+    Proof using.
+    admit.
+    Admitted. *)
+
+      #[global] Instance interp_cfg3_proper_eq_itree {R RR}:
+      Proper (eq_itree eq ==> eq ==> eq ==> eq ==> eq ==> (@eq1 (PropT _) _ _ )) (@interp_cfg3 R RR).
+  Proof.
+    repeat red.
+    intros.
+    subst.
+    admit.
+  Admitted.
+
+    Lemma interp_cfg3_bind' {R S} {RR1} {RR2}:
+    forall t (k : R -> itree _ S) g les sid m,
+    Monad.eq1
+      (interp_cfg3 RR2 (ITree.bind t k) g les sid m)
+          (bind (interp_cfg3 RR1 t g les sid m) (fun '(m',(sid',(les', (g', r)))) => interp_cfg3 RR2 (k r) g' les' sid' m')).
+    Proof.
+    Admitted.
+  Lemma ret_bind': forall {E} (a b : Type) (f : a -> PropT E b) (x : a),
+      eq1 (bind (ret x) f) (f x).
+  Proof using.
+  Admitted.
+#[global] Instance proptT_eq1_proper {E R}:
+  Proper (eq1 ==> eq1 ==> iff) (@eq1 (PropT E) _ R).
+  Proof.
+    repeat red.
+    intros.
+    Admitted.
+  #[global] Instance propT_eq1_eqiv {E R}: Equivalence (@eq1 (PropT E) _ R).
+  Proof.
+    split.
+    + unfold Reflexive.
+      intros.
+      unfold eq1.
+      red.
+      split.
+      - intros.
+        split; intros.
+        admit.
+        admit.
+      - split.
+        unfold eutt_closed.
+        repeat red.
+        intros.
+        split; intros.
+
+
+  Admitted.
+
+
+   #[global] Instance bind_PropT_Proper' {E} {A B} :
+     Proper (eq1 ==> eq ==> (@eq1 (PropT E) _ _)) (@bind_PropT E A B).
+   Proof using.
+   repeat red. intros.
+Admitted.
+Lemma interp3_instr_load _id g les sid mem pointer:
+  (* read_uvalue_spec (DTYPE_I 32)  *)
+  Maps.lookup (Anon 2%Z) les = Some pointer ->
+ eq1 (interp_cfg3 eq (⟦ (IId  _id, (INSTR_Load (DTYPE_I 32) ((DTYPE_Pointer), (EXP_Ident (ID_Local (Anon (2)%Z)))) [ANN_align (4)%Z]))⟧i None) g les sid mem)
+  (MEM_SPEC_INTERP.interp_memory_spec eq 
+    (fmap (fun res => (FMapAList.alist_add _id (dvalue_to_uvalue res) les, (g, tt))) 
+    (ret (DVALUE_None))) sid mem )
+  .
+Proof.
+  simpl.
+  intros.
+  (* split; try reflexivity. *)
+  cbn.
+  rewrite (interp_cfg3_bind' (RR1 := eq)(RR2 := eq)).
+
+  rewrite translate_bind.
+  rewrite (interp_cfg3_bind' (RR1 := eq)(RR2 := eq)).
+  Print bind_bind.
+  rewrite bind_bind_Prop.
+  go.
+  rewrite bind_bind.
+  go.
+  (* rewrite bind_trigger. *)
+  cbn.
+  unfold exp_to_instr.
+  rewrite <- subevent_left.
+  rewrite <- subevent_right.
+  rewrite <- subevent_right.
+  rewrite <- subevent_right.
+  repeat rewrite subevent_subevent.
+  rewrite (interp_cfg3_bind (RR1 := eq)).
+  (* repeat red. *)
+  setoid_rewrite interp_cfg3_LR''; eauto.
+  eapply eq1_iff_propt.
+  rewrite ret_bind.
+  split.
+  intros.
+  split.
+  match goal with 
+    | |- bind ?x ?f => remember x; remember f
+  end.
+  rewrite ret_bind'.
+  setoid_rewrite interp_cfg3_ret.
+  unfold bind.
+  eexists.
+  eexists.
+  rewrite interp_cfg3_LR.
+  Search (vis _ _).
+
+  go.
+  go.
+  process.
+  cbn.
+  eewrite (interp_cfg3_bind (RR1:= eq)).
+  eapply bind_PropT_Proper.
+  repeat red.
+  Check eq1.
+  eapply interp_cfg3_proper.
+  rewrite translate_bind.
+  rewrite translate_bind.
+  unfold interp_cfg3.
+  eapply interp_memory_spec_proper.
+  rewrite interp_intrinsics_bind.
+  reflexivity.
+  reflexivity.
+  remember (interp_local
+(interp_global
+(interp_intrinsics
+(ua <-
+translate exp_to_instr
+(uv <- translate LU_to_exp (trigger (LocalRead (Anon 2%Z)));;
+concretize_if_no_undef_or_poison uv);;
+da <- concretize_or_pick_unique ua;;
+uv <- trigger (Load (DTYPE_I 32) da);; trigger (LocalWrite _id uv))) g) les).
+remember (interp_local
+(interp_global
+(r <-
+interp_intrinsics
+(translate exp_to_instr
+(uv <- translate LU_to_exp (trigger (LocalRead (Anon 2%Z)));;
+concretize_if_no_undef_or_poison uv));;
+interp_intrinsics
+(da <- concretize_or_pick_unique r;;
+uv <- trigger (Load (DTYPE_I 32) da);; trigger (LocalWrite _id uv))) g) les).
+
+  assert (eutt eq i i0).
+  subst.
+  rewrite interp_intrinsics_bind.
+  reflexivity.
+  eapply interp_memory_spec_proper in H0.
+  repeat red in H0.
+  specialize (H0 sid mem).
+  (* destruct H0. *)
+  eapply H0.
+  reflexivity.
+  specialize (H0 i).
+  unfold eq1 in H0.
+  pose proof (@interp_memory_spec_proper).
+
+  reflexivity.
+  reflexivity.
+
+  
+interp_memory_spec eq
+(interp_local
+(interp_global
+(interp_intrinsics
+(ua <-
+translate exp_to_instr
+(uv <- translate LU_to_exp (trigger (LocalRead [...]));;
+concretize_if_no_undef_or_poison uv);;
+da <- concretize_or_pick_unique ua;;
+uv <- trigger (Load (DTYPE_I 32) da);; trigger (LocalWrite _id uv))) g) les) sid mem t'
+
+
+Admitted.
+  (* Lemma denote_instr_load :
+    forall (i : raw_id) volatile τ τp ptr align g l l' m a uv,
+      ⟦ ptr at τp ⟧e3 g l m ≈ Ret3 g l' m (UVALUE_Addr a) ->
+      read m a τ = inr uv ->
+      ⟦ (IId i, INSTR_Load volatile τ (τp, ptr) align) '⟧ i3 g l m ≈ Ret3 g (Maps.add i uv l') m tt.
+  Proof.
+    intros * EXP READ.
+    cbn.
+    go.
+    rewrite EXP.
+    go.
+    cbn.
+    go.
+    step.
+    step.
+    reflexivity.
+  Qed. *)
 
   (* Lemma denote_instr_store : *)
   (*   forall {M} `{MemMonad MemState M} *)
