src/rocq/Theory/InterpreterCFG.v
@@ -10,7 +10,7 @@ From ITree Require Import
      ITree
      Basics.Monad
      Eq.Eqit.
-
+Unset Universe Checking.
 From Vellvm Require Import
      Semantics.
 
@@ -78,13 +78,13 @@ Module CFGTheory (IS : InterpreterStack) (TOP : LLVMTopLevel IS).
     interp_cfg1
     interp_cfg2
     interp_cfg3
-    interp_cfg4
-    interp_cfg5
+    (* interp_cfg4 *)
+    (* interp_cfg5 *)
     interp_mcfg1
     interp_mcfg2
     interp_mcfg3
-    interp_mcfg4
-    interp_mcfg5
+    (* interp_mcfg4 *)
+    (* interp_mcfg5 *)
     : VELLVM_REWRITE.
 
   Import CFGTactics.
